language_formal/spark2014_semantics/wellformedness.v
@@ -42,21 +42,21 @@ Definition binop_type (op: binary_operation) (x y: typ): option typ :=
    - general type check for expressions;
 *)
 Inductive well_typed_expr: symtb -> expr -> typ -> Prop :=
-    | WT_Econst_Int: forall ast_id n tb,
-        well_typed_expr tb (Econst ast_id (Ointconst n)) Tint
-    | WT_Econst_Bool: forall ast_id b tb,
-        well_typed_expr tb (Econst ast_id (Oboolconst b)) Tbool
-    | WT_Evar: forall ast_id x tb m t,
+    | WT_Econst_Int: forall ast_num n tb,
+        well_typed_expr tb (Econst ast_num (Ointconst n)) Tint
+    | WT_Econst_Bool: forall ast_num b tb,
+        well_typed_expr tb (Econst ast_num (Oboolconst b)) Tbool
+    | WT_Evar: forall ast_num x tb m t,
         lookup x tb = Some (m, t) ->  
-        well_typed_expr tb (Evar ast_id x) t
-    | WT_Ebinop: forall ast_id tb op e1 e2 t t1,
+        well_typed_expr tb (Evar ast_num x) t
+    | WT_Ebinop: forall ast_num tb op e1 e2 t t1,
         well_typed_expr tb e1 t ->
         well_typed_expr tb e2 t ->
         binop_type op t t = Some t1 ->
-        well_typed_expr tb (Ebinop ast_id op e1 e2) t1
-    | WT_Eunop: forall ast_id tb op e,
+        well_typed_expr tb (Ebinop ast_num op e1 e2) t1
+    | WT_Eunop: forall ast_num tb op e,
         well_typed_expr tb e Tbool ->
-        well_typed_expr tb (Eunop ast_id op e) Tbool.
+        well_typed_expr tb (Eunop ast_num op e) Tbool.
 
 
 (** ** Well-typed commands *)
@@ -64,25 +64,22 @@ Inductive well_typed_expr: symtb -> expr -> typ -> Prop :=
     - general type checking;
 *)
 Inductive well_typed_stmt: symtb -> stmt  -> Prop :=
-    | WT_Sassign: forall ast_id tb x e m t,
+    | WT_Sassign: forall ast_num tb x e m t,
         lookup x tb = Some (m, t) ->
         well_typed_expr tb e t ->
-        well_typed_stmt tb ((Sassign ast_id x e))
-    | WT_Sseq: forall ast_id c1 c2 tb,
+        well_typed_stmt tb ((Sassign ast_num x e))
+    | WT_Sseq: forall ast_num c1 c2 tb,
         well_typed_stmt tb c1 ->
         well_typed_stmt tb c2 ->
-        well_typed_stmt tb (Sseq ast_id c1 c2)
-    | WT_Sifthen: forall ast_id tb b c,
+        well_typed_stmt tb (Sseq ast_num c1 c2)
+    | WT_Sifthen: forall ast_num tb b c,
         well_typed_expr tb b Tbool ->
         well_typed_stmt tb c ->
-        well_typed_stmt tb (Sifthen ast_id b c)
-    | WT_Swhile: forall ast_id tb b c,
+        well_typed_stmt tb (Sifthen ast_num b c)
+    | WT_Swhile: forall ast_num tb b c,
         well_typed_expr tb b Tbool ->
         well_typed_stmt tb c ->
-        well_typed_stmt tb (Swhile ast_id b c).
-(*    | WT_Sassert: forall ast_id tb e, 
-        well_typed_expr tb e Tbool ->
-        well_typed_stmt tb (Sassert ast_id e) *)
+        well_typed_stmt tb (Swhile ast_num b c).
 
 (* =============================== *)
 
@@ -126,20 +123,20 @@ Function update2 (s: mode_map) (x : idnum) (m: (init_mode * mode)): option mode_
    - all variables used in expression should be in mode _in_ or _in/out_; 
 *)
 Inductive well_defined_expr: mode_map -> expr -> Prop :=
-    | WD_Econst_Int: forall ast_id m n,
-        well_defined_expr m (Econst ast_id (Ointconst n))
-    | WD_Econst_Bool: forall ast_id m b,
-        well_defined_expr m (Econst ast_id (Oboolconst b))
-    | WD_Evar: forall ast_id x m,
-        fetch2 x m = Some (Init, In) \/ fetch2 x m = Some (Init, InOut) ->
-        well_defined_expr m (Evar ast_id x)
-    | WD_Ebinop: forall ast_id m op e1 e2,
+    | WD_Econst_Int: forall ast_num m n,
+        well_defined_expr m (Econst ast_num (Ointconst n))
+    | WD_Econst_Bool: forall ast_num m b,
+        well_defined_expr m (Econst ast_num (Oboolconst b))
+    | WD_Evar: forall ast_num x m md,
+        fetch2 x m = Some (Init, md) -> (* initialized out variables can also be read *)
+        well_defined_expr m (Evar ast_num x)
+    | WD_Ebinop: forall ast_num m op e1 e2,
         well_defined_expr m e1 ->
         well_defined_expr m e2 ->
-        well_defined_expr m (Ebinop ast_id op e1 e2)
-    | WD_Eunop: forall ast_id m op e,
+        well_defined_expr m (Ebinop ast_num op e1 e2)
+    | WD_Eunop: forall ast_num m op e,
         well_defined_expr m e ->
-        well_defined_expr m (Eunop ast_id op e). 
+        well_defined_expr m (Eunop ast_num op e). 
 
 
 (** ** Well-defined commands *)
@@ -152,24 +149,26 @@ Inductive well_defined_expr: mode_map -> expr -> Prop :=
     of the resulting initialization states from both branches;
    - _in/out_ mode checking (for variables that are updated by assignments, their mode should be _out_ or _in\out_);
 *)
+
 Inductive well_defined_stmt: mode_map -> stmt -> mode_map -> Prop :=
-    | WD_Sassign: forall ast_id m m' i x e,
+    | WD_Sassign: forall m e x i md m' ast_num,
         well_defined_expr m e ->
-        fetch2 x m = Some (i, Out) \/ fetch2 x m = Some (i, InOut) ->
-        update2 m x (Init, InOut) = Some m' ->
-        well_defined_stmt m (Sassign ast_id x e) m'
-    | WD_Sseq: forall ast_id c1 c2 m m' m'',
+        fetch2 x m = Some (i, md) ->
+        md <> In ->
+        update2 m x (Init, md) = Some m' ->
+        well_defined_stmt m (Sassign ast_num x e) m'
+    | WD_Sseq: forall ast_num c1 c2 m m' m'',
         well_defined_stmt m c1 m' ->
         well_defined_stmt m' c2 m'' ->
-        well_defined_stmt m (Sseq ast_id c1 c2) m''
-    | WD_Sifthen: forall ast_id m m' b c,
+        well_defined_stmt m (Sseq ast_num c1 c2) m''
+    | WD_Sifthen: forall ast_num m m' b c,
         well_defined_expr m b ->
         well_defined_stmt m c m' ->
-        well_defined_stmt m (Sifthen ast_id b c) m
-    | WD_Swhile: forall ast_id m m' b c,
+        well_defined_stmt m (Sifthen ast_num b c) m
+    | WD_Swhile: forall ast_num m m' b c,
         well_defined_expr m b ->
         well_defined_stmt m c m' ->
-        well_defined_stmt m (Swhile ast_id b c) m.
+        well_defined_stmt m (Swhile ast_num b c) m.
 
 (** ** Lemmas for fetching and updating initialization state *)
 Lemma update2_fetch2: forall s x m s',
@@ -354,7 +353,29 @@ Inductive mode_mapping: symtb -> stack -> (mode_map) -> Prop :=
           mode_mapping tb s ls ->
           mode_mapping ((x, (m, Tint)) :: tb) ((x, Vundef) :: s) ((x, (Uninit, m)) :: ls).
 
-Lemma mode_map_exists: forall tb s,
+Lemma mode_mapping_unique: forall tb s m1 m2,
+    mode_mapping tb s m1 ->
+    mode_mapping tb s m2 ->
+    m1 = m2.
+Proof.
+    intros tb s m1 m2 H.
+    revert m2.
+    induction H;
+    intros m2 H0;
+    inversion H0; subst.
+  - reflexivity.
+  - specialize (IHmode_mapping _ H7); subst.
+    reflexivity.
+  - specialize (IHmode_mapping _ H7); subst; 
+    reflexivity.
+  - specialize (IHmode_mapping _ H6); subst; 
+    reflexivity.
+  - specialize (IHmode_mapping _ H6); subst; 
+    reflexivity.
+Qed.
+
+
+Lemma mode_mapping_exists: forall tb s,
     type_check_stack tb s ->
     exists m, mode_mapping tb s m.
 Proof.
@@ -406,89 +427,89 @@ Qed.
 (* = = = = = = = = = = = = = = = = = = = = = = = = = = = = = = = = *)
 
 (** * Well-Checked *)
-(** get the ast id from the expression ast node *)
-Definition get_ast_id_expr (e: expr): astnum :=
+(** get the ast number from the expression ast node *)
+Definition get_ast_num_expr (e: expr): astnum :=
     match e with
-    | (Econst ast_id n) => ast_id
-    | (Evar ast_id x) => ast_id
-    | (Ebinop ast_id op e1 e2) => ast_id
-    | (Eunop ast_id op e) => ast_id
+    | (Econst ast_num n) => ast_num
+    | (Evar ast_num x) => ast_num
+    | (Ebinop ast_num op e1 e2) => ast_num
+    | (Eunop ast_num op e) => ast_num
     end.
 
-(** get the ast id from the statemet ast node *)
-Definition get_ast_id_stmt (c: stmt): astnum :=
+(** get the ast number from the statemet ast node *)
+Definition get_ast_num_stmt (c: stmt): astnum :=
     match c with
-    | (Sassign ast_id x e) => ast_id
-    | (Sseq ast_id c1 c2) => ast_id
-    | (Sifthen ast_id b c) => ast_id
-    | (Swhile ast_id b c) => ast_id
+    | (Sassign ast_num x e) => ast_num
+    | (Sseq ast_num c1 c2) => ast_num
+    | (Sifthen ast_num b c) => ast_num
+    | (Swhile ast_num b c) => ast_num
     end.
 
-Definition max_id := astnum.
+Definition max_num := astnum.
 
-(** ast_id for each AST node is unique *)
+(** ast_num for each AST node is unique *)
 (** later the ast id will be used to map ast node to the check flag denoting the run-time checks
      that needs to be performed before executing that ast node;
 *)
 
 (** all the ast ids for expression ast nodes are unique: parent node's ast id number is smaller than
      children node's ast id number, and the left child node's id number is smaller than the right child 
-     node's id number; max_id is the maximum ast id number used in the expression
+     node's id number; max_num is the maximum ast id number used in the expression
 *)
-Inductive ast_id_inc_expr: expr -> max_id -> Prop :=
-    | Inc_Econst: forall ast_id n,
-        ast_id_inc_expr (Econst ast_id n) ast_id
-    | Inc_Evar: forall ast_id x,
-        ast_id_inc_expr (Evar ast_id x) ast_id
-    | Inc_Ebinop: forall e1 max1 e2 max2 ast_id1 ast_id2 ast_id op,
-        ast_id_inc_expr e1 max1 ->
-        ast_id_inc_expr e2 max2 ->
-        get_ast_id_expr e1 = ast_id1 ->
-        get_ast_id_expr e2 = ast_id2 ->
-        ast_id < ast_id1 ->
-        ast_id < ast_id2 ->
-        max1 < ast_id2 ->
-        ast_id_inc_expr (Ebinop ast_id op e1 e2) max2
-    | Inc_Eunop: forall e max ast_id0 ast_id op,
-        ast_id_inc_expr e max ->
-        get_ast_id_expr e = ast_id0 ->
-        ast_id < ast_id0 ->
-        ast_id_inc_expr (Eunop ast_id op e) max.
+Inductive ast_num_inc_expr: expr -> max_num -> Prop :=
+    | Inc_Econst: forall ast_num n,
+        ast_num_inc_expr (Econst ast_num n) ast_num
+    | Inc_Evar: forall ast_num x,
+        ast_num_inc_expr (Evar ast_num x) ast_num
+    | Inc_Ebinop: forall e1 max1 e2 max2 ast_num1 ast_num2 ast_num op,
+        ast_num_inc_expr e1 max1 ->
+        ast_num_inc_expr e2 max2 ->
+        get_ast_num_expr e1 = ast_num1 ->
+        get_ast_num_expr e2 = ast_num2 ->
+        ast_num < ast_num1 ->
+        ast_num < ast_num2 ->
+        max1 < ast_num2 ->
+        ast_num_inc_expr (Ebinop ast_num op e1 e2) max2
+    | Inc_Eunop: forall e max ast_num0 ast_num op,
+        ast_num_inc_expr e max ->
+        get_ast_num_expr e = ast_num0 ->
+        ast_num < ast_num0 ->
+        ast_num_inc_expr (Eunop ast_num op e) max.
 
-(** it's similar to ast_id_inc_expr, all ast id number is unique *)
-Inductive ast_id_inc_stmt: stmt -> max_id -> Prop :=
-    | Inc_Sassign: forall e max ast_id0 ast_id x,
-        ast_id_inc_expr e max ->
-        get_ast_id_expr e = ast_id0 ->
-        ast_id < ast_id0 ->
-        ast_id_inc_stmt (Sassign ast_id x e) max
-    | Inc_Sseq: forall c1 max1 c2 max2 ast_id1 ast_id2 ast_id,
-        ast_id_inc_stmt c1 max1 ->
-        ast_id_inc_stmt c2 max2 ->
-        get_ast_id_stmt c1 = ast_id1 ->
-        get_ast_id_stmt c2 = ast_id2 ->
-        ast_id < ast_id1 ->
-        ast_id < ast_id2 ->
-        max1 < ast_id2 ->
-        ast_id_inc_stmt (Sseq ast_id c1 c2) max2
-    | Inc_Sifthen: forall b max1 c max2 ast_id1 ast_id2 ast_id,
-        ast_id_inc_expr b max1 ->
-        ast_id_inc_stmt c max2 ->
-        get_ast_id_expr b = ast_id1 ->
-        get_ast_id_stmt c = ast_id2 ->
-        ast_id < ast_id1 ->
-        ast_id < ast_id2 ->
-        max1 < ast_id2 ->
-        ast_id_inc_stmt (Sifthen ast_id b c) max2
-    | Inc_Swhile: forall b max1 c max2 ast_id1 ast_id2 ast_id,
-        ast_id_inc_expr b max1 ->
-        ast_id_inc_stmt c max2 ->
-        get_ast_id_expr b = ast_id1 ->
-        get_ast_id_stmt c = ast_id2 ->
-        ast_id < ast_id1 -> 
-        ast_id < ast_id2 -> 
-        max1 < ast_id2 ->
-        ast_id_inc_stmt (Swhile ast_id b c) max2.
+(** it's similar to ast_num_inc_expr, all ast id number is unique *)
+Inductive ast_num_inc_stmt: stmt -> max_num -> Prop :=
+    | Inc_Sassign: forall e max ast_num0 ast_num x,
+        ast_num_inc_expr e max ->
+        get_ast_num_expr e = ast_num0 ->
+        ast_num < ast_num0 ->
+        ast_num_inc_stmt (Sassign ast_num x e) max
+    | Inc_Sseq: forall c1 max1 c2 max2 ast_num1 ast_num2 ast_num,
+        ast_num_inc_stmt c1 max1 ->
+        ast_num_inc_stmt c2 max2 ->
+        get_ast_num_stmt c1 = ast_num1 ->
+        get_ast_num_stmt c2 = ast_num2 ->
+        ast_num < ast_num1 ->
+        ast_num < ast_num2 ->
+        max1 < ast_num2 ->
+        ast_num_inc_stmt (Sseq ast_num c1 c2) max2
+    | Inc_Sifthen: forall b max1 c max2 ast_num1 ast_num2 ast_num,
+        ast_num_inc_expr b max1 ->
+        ast_num_inc_stmt c max2 ->
+        get_ast_num_expr b = ast_num1 ->
+        get_ast_num_stmt c = ast_num2 ->
+        ast_num < ast_num1 ->
+        ast_num < ast_num2 ->
+        max1 < ast_num2 ->
+        ast_num_inc_stmt (Sifthen ast_num b c) max2
+    | Inc_Swhile: forall b max1 c max2 ast_num1 ast_num2 ast_num,
+        ast_num_inc_expr b max1 ->
+        ast_num_inc_stmt c max2 ->
+        get_ast_num_expr b = ast_num1 ->
+        get_ast_num_stmt c = ast_num2 ->
+        ast_num < ast_num1 -> 
+        ast_num < ast_num2 -> 
+        max1 < ast_num2 ->
+        ast_num_inc_stmt (Swhile ast_num b c) max2.
 
 
 (** ** Generate the run-time-check flags *)
@@ -507,18 +528,18 @@ Function fetch_ck (id : astnum) (m : check_points): option check_action :=
     end.
 
 (** this's used to constrain that all ast id number used in check_points are smaller than a certain number *)
-Inductive ast_ids_lt: check_points -> astnum -> Prop := 
-    | lt1: forall ls n ast_id ck,
-        ast_ids_lt ls n ->
-        ast_id < n ->
-        ast_ids_lt ((ast_id, ck) ::ls) n
+Inductive ast_nums_lt: check_points -> astnum -> Prop := 
+    | lt1: forall ls n ast_num ck,
+        ast_nums_lt ls n ->
+        ast_num < n ->
+        ast_nums_lt ((ast_num, ck) ::ls) n
     | lt2: forall n,
-        ast_ids_lt nil n.
+        ast_nums_lt nil n.
 
-Lemma ast_ids_lt_trans0: forall ls n n',
-    ast_ids_lt ls n ->
+Lemma ast_nums_lt_trans0: forall ls n n',
+    ast_nums_lt ls n ->
     n <= n' ->
-    ast_ids_lt ls n'.
+    ast_nums_lt ls n'.
 Proof.
     intros ls n n' h1 h2.
     induction h1.
@@ -528,21 +549,21 @@ Proof.
   - constructor.    
 Qed.
 
-Lemma ast_ids_lt_trans: forall ls n n',
-    ast_ids_lt ls n ->
+Lemma ast_nums_lt_trans: forall ls n n',
+    ast_nums_lt ls n ->
     n < n' ->
-    ast_ids_lt ls n'.
+    ast_nums_lt ls n'.
 Proof.
     intros.
-    eapply ast_ids_lt_trans0.
+    eapply ast_nums_lt_trans0.
     apply H. 
     intuition.
 Qed.
 
-Lemma ast_ids_lt_add: forall ast_id n cks flag,
-    ast_id < n ->
-    ast_ids_lt cks n ->
-    ast_ids_lt ((ast_id, flag) :: cks) n.
+Lemma ast_nums_lt_add: forall ast_num n cks flag,
+    ast_num < n ->
+    ast_nums_lt cks n ->
+    ast_nums_lt ((ast_num, flag) :: cks) n.
 Proof.
     intros.
     constructor; auto.
@@ -554,23 +575,23 @@ Qed.
      are stored in a list of type check_points
 *)
 Inductive check_generator_expr: check_points -> expr -> check_points -> Prop :=
-    | CG_Econst: forall ast_id n ls,
-        check_generator_expr ls (Econst ast_id n) ls
-    | CG_Evar: forall ast_id x ls,
-        check_generator_expr ls (Evar ast_id x) ls
-    | CG_Ebinop: forall ls e1 ls1 e2 ls2 ast_id op flag,
-        check_flag (Ebinop ast_id op e1 e2) (Some flag) -> 
-        check_generator_expr ((ast_id, flag) :: ls) e1 ls1 ->
+    | CG_Econst: forall ast_num n ls,
+        check_generator_expr ls (Econst ast_num n) ls
+    | CG_Evar: forall ast_num x ls,
+        check_generator_expr ls (Evar ast_num x) ls
+    | CG_Ebinop: forall ls e1 ls1 e2 ls2 ast_num op flag,
+        check_flag (Ebinop ast_num op e1 e2) (Some flag) -> 
+        check_generator_expr ((ast_num, flag) :: ls) e1 ls1 ->
         check_generator_expr ls1 e2 ls2 ->
-        check_generator_expr ls (Ebinop ast_id op e1 e2) ls2
-    | CG_Ebinop_None: forall ls e1 ls1 e2 ls2 ast_id op,
-        check_flag (Ebinop ast_id op e1 e2) None -> 
+        check_generator_expr ls (Ebinop ast_num op e1 e2) ls2
+    | CG_Ebinop_None: forall ls e1 ls1 e2 ls2 ast_num op,
+        check_flag (Ebinop ast_num op e1 e2) None -> 
         check_generator_expr ls e1 ls1 ->
         check_generator_expr ls1 e2 ls2 ->
-        check_generator_expr ls (Ebinop ast_id op e1 e2) ls2
-    | CG_Eunop: forall ls e ls1 ast_id op,
+        check_generator_expr ls (Ebinop ast_num op e1 e2) ls2
+    | CG_Eunop: forall ls e ls1 ast_num op,
         check_generator_expr ls e ls1 ->
-        check_generator_expr ls (Eunop ast_id op e) ls1.
+        check_generator_expr ls (Eunop ast_num op e) ls1.
 
 (** *** generate run-time-check flags for statements *)
 (** For the SPARK 2014 subset that we are working on, we only consider the division by zero check and 
@@ -578,21 +599,21 @@ Inductive check_generator_expr: check_points -> expr -> check_points -> Prop :=
      checks in the statements in the future. 
  *)
 Inductive check_generator_stmt: check_points -> stmt -> check_points -> Prop :=
-    | CG_Sassign: forall ls1 e ls2 ast_id x,
+    | CG_Sassign: forall ls1 e ls2 ast_num x,
         check_generator_expr ls1 e ls2 ->
-        check_generator_stmt ls1 (Sassign ast_id x e) ls2
-    | CG_Sseq: forall ls1 c1 ls2 c2 ls3 ast_id,
+        check_generator_stmt ls1 (Sassign ast_num x e) ls2
+    | CG_Sseq: forall ls1 c1 ls2 c2 ls3 ast_num,
         check_generator_stmt ls1 c1 ls2 ->
         check_generator_stmt ls2 c2 ls3 ->
-        check_generator_stmt ls1 (Sseq ast_id c1 c2) ls3
-    | CG_Sifthen: forall ls1 b ls2 c ls3 ast_id,
+        check_generator_stmt ls1 (Sseq ast_num c1 c2) ls3
+    | CG_Sifthen: forall ls1 b ls2 c ls3 ast_num,
         check_generator_expr ls1 b ls2 ->
         check_generator_stmt ls2 c ls3 ->
-        check_generator_stmt ls1 (Sifthen ast_id b c) ls3
-    | CG_Swhile: forall ls1 b ls2 c ls3 ast_id,
+        check_generator_stmt ls1 (Sifthen ast_num b c) ls3
+    | CG_Swhile: forall ls1 b ls2 c ls3 ast_num,
         check_generator_expr ls1 b ls2 ->
         check_generator_stmt ls2 c ls3 ->        
-        check_generator_stmt ls1 (Swhile ast_id b c) ls3.
+        check_generator_stmt ls1 (Swhile ast_num b c) ls3.
 
 (** ** Semantics with run-time-checks *)
 (*
@@ -604,45 +625,45 @@ Inductive correct_flag_on_op: check_action -> binary_operation -> Prop :=
      whether a check is needed to be performed before executing the expression ast node
 *)
 Inductive eval_expr_with_checks (cps: check_points): stack -> expr -> return_val -> Prop :=
-    | eval_Const: forall cst v s ast_id,
+    | eval_Const: forall cst v s ast_num,
         eval_constant cst = v ->
-        eval_expr_with_checks cps s (Econst ast_id cst) (ValNormal v)
-    | eval_Var: forall x s v ast_id,
+        eval_expr_with_checks cps s (Econst ast_num cst) (ValNormal v)
+    | eval_Var: forall x s v ast_num,
         fetch x s = Some v ->
-        eval_expr_with_checks cps s (Evar ast_id x) (ValNormal v)
-    | eval_Binop1: forall s e1 ast_id op e2,
+        eval_expr_with_checks cps s (Evar ast_num x) (ValNormal v)
+    | eval_Binop1: forall s e1 ast_num op e2,
         eval_expr_with_checks cps s e1 ValException ->
-        eval_expr_with_checks cps s (Ebinop ast_id op e1 e2) ValException
-    | eval_Binop2: forall s e1 v1 e2 ast_id op,
+        eval_expr_with_checks cps s (Ebinop ast_num op e1 e2) ValException
+    | eval_Binop2: forall s e1 v1 e2 ast_num op,
         eval_expr_with_checks cps s e1 (ValNormal v1) ->
         eval_expr_with_checks cps s e2 ValException ->
-        eval_expr_with_checks cps s (Ebinop ast_id op e1 e2) ValException
-    | eval_Binop3: forall s e1 v1 e2 v2 ck ast_id op,
+        eval_expr_with_checks cps s (Ebinop ast_num op e1 e2) ValException
+    | eval_Binop3: forall s e1 v1 e2 v2 ck ast_num op,
         eval_expr_with_checks cps s e1 (ValNormal v1) ->
         eval_expr_with_checks cps s e2 (ValNormal v2) ->
-        fetch_ck ast_id cps = Some ck ->
+        fetch_ck ast_num cps = Some ck ->
         do_check op v1 v2 false ->
-        eval_expr_with_checks cps s (Ebinop ast_id op e1 e2) ValException
-    | eval_Binop4: forall s e1 v1 e2 v2 ck ast_id op v,
+        eval_expr_with_checks cps s (Ebinop ast_num op e1 e2) ValException
+    | eval_Binop4: forall s e1 v1 e2 v2 ck ast_num op v,
         eval_expr_with_checks cps s e1 (ValNormal v1) ->
         eval_expr_with_checks cps s e2 (ValNormal v2) ->
-        fetch_ck ast_id cps = Some ck -> 
+        fetch_ck ast_num cps = Some ck -> 
         do_check op v1 v2 true ->
         eval_binexpr op v1 v2 v ->
-        eval_expr_with_checks cps s (Ebinop ast_id op e1 e2) (ValNormal v)
-    | eval_Binop5: forall s e1 v1 e2 v2 ast_id op v,
+        eval_expr_with_checks cps s (Ebinop ast_num op e1 e2) (ValNormal v)
+    | eval_Binop5: forall s e1 v1 e2 v2 ast_num op v,
         eval_expr_with_checks cps s e1 (ValNormal v1) ->
         eval_expr_with_checks cps s e2 (ValNormal v2) ->
-        fetch_ck ast_id cps = None ->
+        fetch_ck ast_num cps = None ->
         eval_binexpr op v1 v2 v ->
-        eval_expr_with_checks cps s (Ebinop ast_id op e1 e2) (ValNormal v)
-    | eval_Unop1: forall s e ast_id op,
+        eval_expr_with_checks cps s (Ebinop ast_num op e1 e2) (ValNormal v)
+    | eval_Unop1: forall s e ast_num op,
         eval_expr_with_checks cps s e ValException ->
-        eval_expr_with_checks cps s (Eunop ast_id op e) ValException
-    | eval_Unop2: forall s e v ast_id op v1,
+        eval_expr_with_checks cps s (Eunop ast_num op e) ValException
+    | eval_Unop2: forall s e v ast_num op v1,
         eval_expr_with_checks cps s e (ValNormal v) ->
         eval_unaryexpr op v v1 ->
-        eval_expr_with_checks cps s (Eunop ast_id op e) (ValNormal v1).
+        eval_expr_with_checks cps s (Eunop ast_num op e) (ValNormal v1).
 
 
 (** 
@@ -651,45 +672,45 @@ Inductive eval_expr_with_checks (cps: check_points): stack -> expr -> return_val
     for expressions, and there are checks enfornced on the statements
 *)
 Inductive eval_stmt_with_checks (cps: check_points): stack -> stmt -> state -> Prop :=
-    | eval_Assign1: forall s e ast_id x,
+    | eval_Assign1: forall s e ast_num x,
         eval_expr_with_checks cps s e ValException ->
-        eval_stmt_with_checks cps s (Sassign ast_id x e) SException
-    | eval_Assign2: forall s e v x s1 ast_id,
+        eval_stmt_with_checks cps s (Sassign ast_num x e) SException
+    | eval_Assign2: forall s e v x s1 ast_num,
         eval_expr_with_checks cps s e (ValNormal v) ->
         update s x (Value v) = Some s1 -> 
-        eval_stmt_with_checks cps s (Sassign ast_id x e) (SNormal s1)
-    | eval_Seq1: forall s c1 ast_id c2,
+        eval_stmt_with_checks cps s (Sassign ast_num x e) (SNormal s1)
+    | eval_Seq1: forall s c1 ast_num c2,
         eval_stmt_with_checks cps s c1 SException ->
-        eval_stmt_with_checks cps s (Sseq ast_id c1 c2) SException
-    | eval_Seq2: forall ast_id s s1 s2 c1 c2,
+        eval_stmt_with_checks cps s (Sseq ast_num c1 c2) SException
+    | eval_Seq2: forall ast_num s s1 s2 c1 c2,
         eval_stmt_with_checks cps s c1 (SNormal s1) ->
         eval_stmt_with_checks cps s1 c2 s2 ->
-        eval_stmt_with_checks cps s (Sseq ast_id c1 c2) s2
-    | eval_Ifthen: forall s b ast_id c,
+        eval_stmt_with_checks cps s (Sseq ast_num c1 c2) s2
+    | eval_Ifthen: forall s b ast_num c,
         eval_expr_with_checks cps s b ValException ->
-        eval_stmt_with_checks cps s (Sifthen ast_id b c) SException
-    | eval_Ifthen_True: forall s b c s1 ast_id,
+        eval_stmt_with_checks cps s (Sifthen ast_num b c) SException
+    | eval_Ifthen_True: forall s b c s1 ast_num,
         eval_expr_with_checks cps s b (ValNormal (Bool true)) ->
         eval_stmt_with_checks cps s c s1 ->
-        eval_stmt_with_checks cps s (Sifthen ast_id b c) s1
-    | eval_Ifthen_False: forall s b ast_id c,
+        eval_stmt_with_checks cps s (Sifthen ast_num b c) s1
+    | eval_Ifthen_False: forall s b ast_num c,
         eval_expr_with_checks cps s b (ValNormal (Bool false)) ->
-        eval_stmt_with_checks cps s (Sifthen ast_id b c) (SNormal s)
-    | eval_While: forall s b ast_id c,
+        eval_stmt_with_checks cps s (Sifthen ast_num b c) (SNormal s)
+    | eval_While: forall s b ast_num c,
         eval_expr_with_checks cps s b ValException ->
-        eval_stmt_with_checks cps s (Swhile ast_id b c) SException
-    | eval_While_True1: forall s b c ast_id,
+        eval_stmt_with_checks cps s (Swhile ast_num b c) SException
+    | eval_While_True1: forall s b c ast_num,
         eval_expr_with_checks cps s b (ValNormal (Bool true)) ->
         eval_stmt_with_checks cps s c SException ->
-        eval_stmt_with_checks cps s (Swhile ast_id b c) SException
-    | eval_While_True2: forall s b c s1 ast_id s2,
+        eval_stmt_with_checks cps s (Swhile ast_num b c) SException
+    | eval_While_True2: forall s b c s1 ast_num s2,
         eval_expr_with_checks cps s b (ValNormal (Bool true)) ->
         eval_stmt_with_checks cps s c (SNormal s1) ->
-        eval_stmt_with_checks cps s1 (Swhile ast_id b c) s2 ->
-        eval_stmt_with_checks cps s (Swhile ast_id b c) s2
-    | eval_While_False: forall s b ast_id c,
+        eval_stmt_with_checks cps s1 (Swhile ast_num b c) s2 ->
+        eval_stmt_with_checks cps s (Swhile ast_num b c) s2
+    | eval_While_False: forall s b ast_num c,
         eval_expr_with_checks cps s b (ValNormal (Bool false)) ->
-        eval_stmt_with_checks cps s (Swhile ast_id b c) (SNormal s).
+        eval_stmt_with_checks cps s (Swhile ast_num b c) (SNormal s).
 
 
 (** some basic lemmas *)
@@ -708,13 +729,13 @@ Qed.
 
 (** 
    the ast id number is increasing: parent node's ast id number is smaller than children node's ast id number.
-   (get_ast_id_expr e) is the ast id number for expression e, and max is the maximum ast id number used 
-   by e. if e has no subexpression, then max is the same as (get_ast_id_expr e), otherwise, max is maximum
-   ast id number of its subexpressions, so (get_ast_id_expr e) should be less and equal max
+   (get_ast_num_expr e) is the ast id number for expression e, and max is the maximum ast id number used 
+   by e. if e has no subexpression, then max is the same as (get_ast_num_expr e), otherwise, max is maximum
+   ast id number of its subexpressions, so (get_ast_num_expr e) should be less and equal max
 *)
-Lemma ast_id_bound_expr: forall e max,
-    ast_id_inc_expr e max ->
-    get_ast_id_expr e <= max.
+Lemma ast_num_bound_expr: forall e max,
+    ast_num_inc_expr e max ->
+    get_ast_num_expr e <= max.
 Proof.
     intros e max h.
     induction h; simpl; intuition.
@@ -725,79 +746,79 @@ Qed.
     the results are stored in cks indexed by expression and its subexpression ast ids,
     because max is the maximum ast id, so all ast ids in cks should be less than (max + 1)
 *)
-Lemma ast_id_max_expr: forall e max cks0 cks,
-    ast_id_inc_expr e max ->
+Lemma ast_num_max_expr: forall e max cks0 cks,
+    ast_num_inc_expr e max ->
     check_generator_expr cks0 e cks ->
-    ast_ids_lt cks0 (get_ast_id_expr e) ->
-    ast_ids_lt cks (max + 1).
+    ast_nums_lt cks0 (get_ast_num_expr e) ->
+    ast_nums_lt cks (max + 1).
 Proof.
     intros e max cks0 cks h1.
     revert cks0 cks.
     induction h1;
     intros cks0 cks h2 h3;
     simpl in h3; inversion h2; subst.
-  - apply ast_ids_lt_trans with (n := ast_id); intuition.
-  - apply ast_ids_lt_trans with (n := ast_id); intuition.
-  - specialize (ast_ids_lt_trans _ _ _ h3 H1); intros hz1.
-    specialize (ast_ids_lt_add _ _ _ flag H1 hz1); intros hz2.
+  - apply ast_nums_lt_trans with (n := ast_num); intuition.
+  - apply ast_nums_lt_trans with (n := ast_num); intuition.
+  - specialize (ast_nums_lt_trans _ _ _ h3 H1); intros hz1.
+    specialize (ast_nums_lt_add _ _ _ flag H1 hz1); intros hz2.
     specialize (IHh1_1 _ _ H11 hz2).
-    assert(hz: max1 + 1 <= get_ast_id_expr e2); intuition.
-    specialize (ast_ids_lt_trans0 _ _ _ IHh1_1 hz); intros hz3.
+    assert(hz: max1 + 1 <= get_ast_num_expr e2); intuition.
+    specialize (ast_nums_lt_trans0 _ _ _ IHh1_1 hz); intros hz3.
     specialize (IHh1_2 _ _ H12 hz3).
     assumption.
-  - specialize (ast_ids_lt_trans _ _ _ h3 H1); intros hz1.
+  - specialize (ast_nums_lt_trans _ _ _ h3 H1); intros hz1.
     specialize (IHh1_1 _ _ H11 hz1).
-    assert(hz: max1 + 1 <= get_ast_id_expr e2); intuition.
-    specialize (ast_ids_lt_trans0 _ _ _ IHh1_1 hz); intros hz3.
+    assert(hz: max1 + 1 <= get_ast_num_expr e2); intuition.
+    specialize (ast_nums_lt_trans0 _ _ _ IHh1_1 hz); intros hz3.
     specialize (IHh1_2 _ _ H12 hz3).
     assumption.
-  - specialize (ast_ids_lt_trans _ _ _ h3 H0); intros hz1.
+  - specialize (ast_nums_lt_trans _ _ _ h3 H0); intros hz1.
     specialize (IHh1 _ _ H5 hz1).
     assumption.
 Qed.
 
-(** it's similar to ast_id_bound_expr *)
-Lemma ast_id_bound_stmt: forall c max,
-    ast_id_inc_stmt c max ->
-    get_ast_id_stmt c <= max.
+(** it's similar to ast_num_bound_expr *)
+Lemma ast_num_bound_stmt: forall c max,
+    ast_num_inc_stmt c max ->
+    get_ast_num_stmt c <= max.
 Proof.
     intros c max h.
     induction h; simpl; intuition.
-    specialize (ast_id_bound_expr _ _ H); intros hz1.
+    specialize (ast_num_bound_expr _ _ H); intros hz1.
     intuition.    
 Qed.
 
-(** it's similar to ast_id_max_expr *)
-Lemma ast_id_max_stmt: forall c max cks0 cks1,
-    ast_id_inc_stmt c max ->
+(** it's similar to ast_num_max_expr *)
+Lemma ast_num_max_stmt: forall c max cks0 cks1,
+    ast_num_inc_stmt c max ->
     check_generator_stmt cks0 c cks1 ->
-    ast_ids_lt cks0 (get_ast_id_stmt c) ->
-    ast_ids_lt cks1 (max + 1).
+    ast_nums_lt cks0 (get_ast_num_stmt c) ->
+    ast_nums_lt cks1 (max + 1).
 Proof.
     intros c max cks0 cks1 h1.
     revert cks0 cks1.
     induction h1;
     intros cks0 cks1 h2 h3;
     simpl in h3; inversion h2; subst.
-  - specialize (ast_ids_lt_trans _ _ _ h3 H1); intros hz1.
-    specialize (ast_id_max_expr _ _ _ _ H H7 hz1); intros hz2.
+  - specialize (ast_nums_lt_trans _ _ _ h3 H1); intros hz1.
+    specialize (ast_num_max_expr _ _ _ _ H H7 hz1); intros hz2.
     assumption.
-  - specialize (ast_ids_lt_trans _ _ _ h3 H1); intros hz1.
+  - specialize (ast_nums_lt_trans _ _ _ h3 H1); intros hz1.
     specialize (IHh1_1 _ _ H9 hz1).
-    assert (hz: max1 + 1 <= get_ast_id_stmt c2); intuition.
-    specialize (ast_ids_lt_trans0 _ _ _ IHh1_1 hz); intros hz2.
+    assert (hz: max1 + 1 <= get_ast_num_stmt c2); intuition.
+    specialize (ast_nums_lt_trans0 _ _ _ IHh1_1 hz); intros hz2.
     specialize (IHh1_2 _ _ H10 hz2).
     assumption.
-  - specialize (ast_ids_lt_trans _ _ _ h3 H2); intros hz1.
-    specialize (ast_id_max_expr _ _ _ _ H H10 hz1); intros hz2.
-    assert (hz: max1 + 1 <= get_ast_id_stmt c); intuition.
-    specialize (ast_ids_lt_trans0 _ _ _ hz2 hz); intros hz3.
+  - specialize (ast_nums_lt_trans _ _ _ h3 H2); intros hz1.
+    specialize (ast_num_max_expr _ _ _ _ H H10 hz1); intros hz2.
+    assert (hz: max1 + 1 <= get_ast_num_stmt c); intuition.
+    specialize (ast_nums_lt_trans0 _ _ _ hz2 hz); intros hz3.
     specialize (IHh1 _ _ H11 hz3).
     assumption.
-  - specialize (ast_ids_lt_trans _ _ _ h3 H2); intros hz1.
-    specialize (ast_id_max_expr _ _ _ _ H H10 hz1); intros hz2.
-    assert (hz: max1 + 1 <= get_ast_id_stmt c); intuition.
-    specialize (ast_ids_lt_trans0 _ _ _ hz2 hz); intros hz3.
+  - specialize (ast_nums_lt_trans _ _ _ h3 H2); intros hz1.
+    specialize (ast_num_max_expr _ _ _ _ H H10 hz1); intros hz2.
+    assert (hz: max1 + 1 <= get_ast_num_stmt c); intuition.
+    specialize (ast_nums_lt_trans0 _ _ _ hz2 hz); intros hz3.
     specialize (IHh1 _ _ H11 hz3).
     assumption.
 Qed.
